ImpE2.v
@@ -1,0 +1,529 @@
+(* FIXME: Copied these from pset4; probably won't need all of them. *)
+
+Require Import Bool Arith List Omega ListSet.
+Require Import Recdef Morphisms.
+Require Import Program.Tactics.
+Require Import Relation_Operators.
+Require FMapList.
+Require FMapFacts.
+Require Import Classical.
+Require Import Coq.Classes.RelationClasses.
+Require Import OrderedType OrderedTypeEx DecidableType.
+Require Import Coq.Logic.FunctionalExtensionality.
+Require Import Sorting.Permutation.
+Import ListNotations.
+Require Import Common.
+(* XXX NOTE: name conflicts will occur *)
+Require Import ImpE.
+
+(*******************************************************************************
+*
+* SYNTAX
+*
+*******************************************************************************)
+
+Section Syntax.
+  Inductive exp2 : Type :=
+  | Enat2 : nat -> exp2
+  | Evar2 : var -> exp2
+  | Eplus2 : exp2 -> exp2 -> exp2
+  | Emult2 : exp2 -> exp2 -> exp2
+  | Eloc2 : location -> exp2
+  | Ederef2 : exp2 -> exp2
+  | Eisunset2 : condition -> exp2
+  | Elambda2 : mode -> com2 -> exp2
+                                   
+  with com2 : Type :=
+  | Cskip2 : com2
+  | Cassign2 : var -> exp2 -> com2
+  | Cdeclassify2 : var -> exp2 -> com2
+  | Cupdate2 : exp2 -> exp2 -> com2
+  | Coutput2 : exp2 -> sec_level -> com2
+  | Ccall2 : exp2 -> com2
+  | Cset2 : condition -> com2
+  | Cenclave2 : enclave -> com2 -> com2
+  | Ckill2 : enclave -> com2
+  | Cseq2 : list com2 -> com2
+  | Cif2 : exp2 -> com2 -> com2 -> com2
+  | Cwhile2 : exp2 -> com2 -> com2.
+
+  Inductive val2 : Type :=
+  | Vlambda2 : mode -> com2 -> val2
+  | Vnat2 : nat -> val2
+  | Vloc2 : location -> val2
+  | Vpair2 : val2 -> val2 -> val2.
+
+  Function forall_subexp2 (e: exp2) (P: exp2 -> Prop) : Prop :=
+    P e /\
+    match e with
+    | Eplus2 e1 e2 => forall_subexp2 e1 P /\ forall_subexp2 e2 P
+    | Emult2 e1 e2 => forall_subexp2 e1 P /\ forall_subexp2 e2 P
+    | Ederef2 e' => forall_subexp2 e' P
+    | Elambda2 _ c => forall_subexp2' c P
+    | _ => True
+    end
+  with forall_subexp2' (c: com2) (P: exp2 -> Prop) : Prop :=
+    match c with
+    | Cassign2 _ e => forall_subexp2 e P
+    | Cdeclassify2 _ e => forall_subexp2 e P
+    | Cupdate2 e1 e2 => forall_subexp2 e1 P /\ forall_subexp2 e2 P
+    | Ccall2 e => forall_subexp2 e P
+    | Cenclave2 _ c' => forall_subexp2' c' P
+    | Cseq2 cs => fold_left (fun acc c => forall_subexp2' c P /\ acc) cs True
+    | Cif2 e c1 c2 =>
+      forall_subexp2 e P /\ forall_subexp2' c1 P /\ forall_subexp2' c2 P
+    | Cwhile2 e c' => forall_subexp2 e P /\ forall_subexp2' c' P
+    | _ => True
+    end.
+
+  Definition exp2_novars (e: exp2) : Prop :=
+    forall_subexp2 e (fun e =>
+                       match e with
+                       | Evar2 _ => False
+                       | _ => True
+                       end).
+End Syntax.
+
+(*******************************************************************************
+*
+* SEMANTICS
+*
+*******************************************************************************)
+
+Section Semantics.
+  Definition reg2 : Type := register val2.
+  Definition reg_init2 : reg2 := fun x => Vnat2 0.
+  Definition mem2 : Type := memory val2.
+  Inductive kill2 : Type :=
+  | Single: set enclave -> kill2
+  | Pair: (set enclave * set enclave) -> kill2.
+
+  Inductive event2 : Type :=
+  | Decl : exp2 -> mem2 -> event2
+  | Mem : mem2 -> event2
+  | Out : sec_level -> val2 -> event2.
+  Definition trace2 : Type := list event2.
+
+  (* XXX TODO LYT
+  Definition merge_reg (r1 r2: reg2) := .
+  Definition merge_kill (k1 k2: set enclave) := .
+  Definition merge_mem (m1 m2: mem2) := .
+  Definition merge_trace (t1 t2: trace2) := .
+*)  
+
+  Definition econfig2 : Type := exp2 * reg2 * mem2 * kill2.
+  Definition ecfg_exp2 (ecfg: econfig2) : exp2 :=
+    match ecfg with (e, _, _, _) => e end.
+  Definition ecfg_reg2 (ecfg: econfig2) : reg2 :=
+    match ecfg with (_, r, _, _) => r end.
+  Definition ecfg_update_exp2 (ecfg: econfig2) (e: exp2) : econfig2 :=
+    match ecfg with (_, r, m, k) => (e, r, m, k) end.
+  Definition esemantics2 : Type := mode -> loc_mode -> econfig2 -> val2 -> Prop.
+
+  Inductive estep2 : esemantics2 :=
+  | Estep2_nat : forall md d ecfg n,
+      ecfg_exp2 ecfg = Enat2 n ->
+      estep2 md d ecfg (Vnat2 n)
+  | Estep2_loc : forall md d ecfg l,
+      ecfg_exp2 ecfg = Eloc2 l ->
+      estep2 md d ecfg (Vloc2 l)
+  | Estep2_lambda : forall md d ecfg c,
+      ecfg_exp2 ecfg = Elambda2 md c ->
+      estep2 md d ecfg (Vlambda2 md c)
+  | Estep2_var : forall md d ecfg x v,
+      ecfg_exp2 ecfg = Evar2 x ->
+      ecfg_reg ecfg x = v ->
+      estep2 md d ecfg v
+  | Estep2_plus : forall md d ecfg e1 e2 n1 n2,
+      ecfg_exp2 ecfg = Eplus e1 e2 ->
+      estep2 md d (ecfg_update_exp2 ecfg e1) (Vnat2 n1) ->
+      estep2 md d (ecfg_update_exp2 ecfg e2) (Vnat2 n2) ->
+      estep2 md d ecfg (Vnat (n1 + n2))
+  | Estep2_mult : forall md d ecfg e1 e2 n1 n2,
+      ecfg_exp2 ecfg = Emult e1 e2 ->
+      estep2 md d (ecfg_update_exp2 ecfg e1) (Vnat2 n1) ->
+      estep2 md d (ecfg_update_exp2 ecfg e2) (Vnat2 n2) ->
+      estep2 md d ecfg (Vnat (n1 * n2))
+  | Estep2_deref : forall md d ecfg e r m k l v,
+      ecfg = (Ederef e, r, m, k) ->
+      estep2 md d (e, r, m, k) (Vloc l) ->
+      m l = v ->
+      mode_access_ok md d l k ->
+      estep2 md d ecfg v
+  | Estep2_isunset : forall md d ecfg cnd v res,
+      ecfg_exp2 ecfg = Eisunset cnd ->
+      estep2 md d (ecfg_update_exp2 ecfg (Ederef (Eloc (Cnd cnd)))) v ->
+      (v = Vnat 0 /\ res = Vnat 1) \/ (v <> Vnat 0 /\ res = Vnat 0) ->
+      estep2 md d ecfg res.
+
+  (* Semantics for commands. *)
+  Definition cconfig : Type := com2 * reg * mem * set enclave.
+  Definition cterm : Type := reg * mem * set enclave.
+  Definition ccfg_com2 (ccfg: cconfig) : com2 :=
+    match ccfg with (c, _, _, _) => c end.
+  Definition ccfg_reg (ccfg: cconfig) : reg :=
+    match ccfg with (_, r, _, _) => r end.
+  Definition ccfg_mem (ccfg: cconfig) : mem :=
+    match ccfg with (_, _, m, _) => m end.
+  Definition ccfg_kill (ccfg: cconfig) : set enclave :=
+    match ccfg with (_, _, _, k) => k end.
+  Definition ccfg_update_mem (ccfg: cconfig) (l: location) (v: val) : mem := 
+    fun loc => if locations_eq loc l then v
+               else (ccfg_mem ccfg) loc.
+  Definition ccfg_update_reg (ccfg: cconfig) (x: var) (v: val) : reg :=
+    fun var => if var =? x then v
+               else (ccfg_reg ccfg) var.
+  Definition ccfg_to_ecfg (e: exp2) (ccfg : cconfig) : econfig :=
+    (e, (ccfg_reg ccfg), (ccfg_mem ccfg), (ccfg_kill ccfg)).
+  Definition ccfg_update_com2 (c: com2) (ccfg : cconfig) : cconfig :=
+    (c, (ccfg_reg ccfg), (ccfg_mem ccfg), (ccfg_kill ccfg)).
+  Definition csemantics : Type := mode -> loc_mode -> cconfig -> cterm -> trace -> Prop.  
+
+  (* XXX couldn't figure out a way to not have to introduce forall md d ccfg everywhere.. *)
+  Inductive cstep : csemantics := 
+  | Cstep_skip : forall md d ccfg, cstep md d ccfg (ccfg_reg ccfg, ccfg_mem ccfg, ccfg_kill ccfg) []
+  | Cstep_assign : forall md d ccfg x e v r',
+      ccfg_com2 ccfg = Cassign x e ->
+      estep2 md d (ccfg_to_ecfg e ccfg) v ->
+      r' = ccfg_update_reg ccfg x v ->
+      mode_alive md (ccfg_kill ccfg) ->
+      cstep md d ccfg (r', ccfg_mem ccfg, ccfg_kill ccfg) []
+  | Cstep_declassify : forall md d ccfg x e v r',
+      ccfg_com2 ccfg = Cdeclassify x e ->
+      exp2_novars e ->
+      estep2 md d (ccfg_to_ecfg e ccfg) v ->
+      r' = ccfg_update_reg ccfg x v ->
+      mode_alive md (ccfg_kill ccfg) ->
+      cstep md d ccfg (r', ccfg_mem ccfg, ccfg_kill ccfg) [Decl e (ccfg_mem ccfg)]
+  | Cstep_update : forall md d ccfg e1 e2 l v m',
+      ccfg_com2 ccfg = Cupdate e1 e2 ->
+      estep2 md d (ccfg_to_ecfg e1 ccfg) (Vloc l) ->
+      estep2 md d (ccfg_to_ecfg e2 ccfg) v ->
+      mode_alive md (ccfg_kill ccfg) ->
+      mode_access_ok md d l (ccfg_kill ccfg) ->
+      is_Not_cnd l ->
+      m' = ccfg_update_mem ccfg l v ->
+      cstep md d ccfg (ccfg_reg ccfg, m', ccfg_kill ccfg) []
+  | Cstep_output : forall md d ccfg e sl v,
+      ccfg_com2 ccfg = Coutput e sl ->
+      estep2 md d (ccfg_to_ecfg e ccfg) v ->
+      sl = L \/ sl = H ->
+      mode_alive md (ccfg_kill ccfg) ->
+      cstep md d ccfg (ccfg_reg ccfg, ccfg_mem ccfg, ccfg_kill ccfg) [Mem (ccfg_mem ccfg); Out sl v]
+  | Cstep_call : forall md d ccfg e c r' m' k' tr,
+      ccfg_com2 ccfg = Ccall e ->
+      estep2 md d (ccfg_to_ecfg e ccfg) (Vlambda md c) ->
+      cstep md d (ccfg_update_com2 c ccfg) (r', m', k') tr ->
+      cstep md d ccfg (r', m', k') tr
+  | Cstep_cset : forall md d ccfg c m',
+      ccfg_com2 ccfg = Cset c ->
+      mode_access_ok md d (Cnd c) (ccfg_kill ccfg) ->
+      m' = ccfg_update_mem ccfg (Cnd c) (Vnat 1) ->
+      mode_alive md (ccfg_kill ccfg) ->
+      cstep md d ccfg (ccfg_reg ccfg, m', ccfg_kill ccfg) [Mem m']
+  | Cstep_enclave : forall md d ccfg enc c r' m' k' tr,
+    md = Normal ->
+    ccfg_com2 ccfg = Cenclave enc c ->
+    cstep (Encl enc) d (c, ccfg_reg ccfg, ccfg_mem ccfg, ccfg_kill ccfg) (r', m', k') tr ->
+    cstep md d ccfg (r', m', k') tr
+  | Cstep_seq_nil : forall md d ccfg,
+      ccfg_com2 ccfg = Cseq [] ->
+      cstep md d ccfg (ccfg_reg ccfg, ccfg_mem ccfg, ccfg_kill ccfg) []
+  | Cstep_seq_hd : forall md d ccfg hd tl r m k tr r' m' k' tr',
+      ccfg_com2 ccfg = Cseq (hd::tl) ->
+      cstep md d (ccfg_update_com2 hd ccfg) (r, m, k) tr ->
+      cstep md d (Cseq tl, r, m, k) (r', m', k') tr' ->
+      cstep md d ccfg (r', m', k') (tr++tr')
+  | Cstep_if : forall md d ccfg e c1 c2 v r' m' k' tr,
+      ccfg_com2 ccfg = Cif e c1 c2 ->
+      estep2 md d (ccfg_to_ecfg e ccfg) v ->
+      ~(v = (Vnat 0)) ->
+      cstep md d (ccfg_update_com2 c1 ccfg) (r', m', k') tr ->
+      cstep md d ccfg (r', m', k') tr
+  | Cstep_else : forall md d ccfg e c1 c2 v r' m' k' tr,
+      ccfg_com2 ccfg = Cif e c1 c2 ->
+      estep2 md d (ccfg_to_ecfg e ccfg) v ->
+      v = (Vnat 0) ->
+      cstep md d (ccfg_update_com2 c2 ccfg) (r', m', k') tr ->
+      cstep md d ccfg (r', m', k') tr
+  | Cstep_while_t : forall md d ccfg e c v r m k tr r' m' k' tr',
+      ccfg_com2 ccfg = Cwhile e c ->
+      estep2 md d (ccfg_to_ecfg e ccfg) v ->
+      ~(v = (Vnat 0)) ->
+      cstep md d (ccfg_update_com2 c ccfg) (r, m, k) tr ->
+      cstep md d (ccfg_update_com2 (Cwhile e c) ccfg) (r', m', k') tr' ->
+      cstep md d ccfg (r', m', k') (tr++tr')
+  | Cstep_while_f : forall md d ccfg e c,
+      ccfg_com2 ccfg = Cwhile e c ->
+      estep2 md d (ccfg_to_ecfg e ccfg) (Vnat 0) ->
+      mode_alive md (ccfg_kill ccfg) ->
+      cstep md d ccfg (ccfg_reg ccfg, ccfg_mem ccfg, ccfg_kill ccfg) []
+  | Cstep_kill : forall md d ccfg enc,
+      md = Normal ->
+      ccfg_com2 ccfg = Ckill enc ->
+      mode_alive (Encl enc) (ccfg_kill ccfg) ->
+      cstep md d ccfg (ccfg_reg ccfg, ccfg_mem ccfg, set_add Nat.eq_dec enc (ccfg_kill ccfg)) [].
+  
+End Semantics.
+
+(*******************************************************************************
+*
+* TYPING
+*
+*******************************************************************************)
+
+Section Typing.
+  Inductive ref_type : Set :=
+  | Mut
+  | Immut.
+
+  (* FIXME: we might want to change contexts to be defined in terms of
+     finite maps instead of functions. *)
+  Inductive base_type : Type :=
+  | Tnat : base_type
+  | Tcond : mode -> base_type
+  | Tref : type -> mode -> ref_type -> base_type
+  | Tlambda (G: context) (k:set enclave) (u:set condition) (p: sec_policy)
+            (md: mode) (G': context) (k':set enclave) : base_type
+                           
+  with type : Type :=
+  | Typ : base_type -> sec_policy -> type
+                                            
+  with context : Type :=
+  | Cntxt (var_cntxt: var -> option type)
+          (loc_cntxt: location -> option (type * ref_type)) : context.
+                                      
+  Definition var_context (G: context) : var -> option type :=
+    match G with Cntxt vc _ => vc end.
+  
+  Definition loc_context (G: context) : location -> option (type * ref_type) :=
+    match G with Cntxt _ lc => lc end.
+
+  Inductive var_in_dom (G: context) : var -> type -> Prop :=
+  | Var_in_dom : forall x t,
+      var_context G x = Some t ->
+      var_in_dom G x t.
+
+  Inductive loc_in_dom (G: context) : location -> type -> ref_type -> Prop :=
+  | Loc_in_dom : forall l t rt,
+      loc_context G l = Some (t, rt) ->
+      loc_in_dom G l t rt.
+
+  Definition forall_var (G: context) (P: var -> type -> Prop) : Prop :=
+    forall x t, var_in_dom G x t -> P x t.
+
+  Definition forall_loc (G: context)
+             (P: location -> type -> ref_type -> Prop) : Prop :=
+    forall l t rt,
+      loc_in_dom G l t rt -> P l t rt.
+
+  Definition forall_dom (G: context)
+             (P: var -> type -> Prop)
+             (Q: location -> type -> ref_type -> Prop) : Prop :=
+    forall_var G P /\ forall_loc G Q.
+
+  Inductive type_le : type -> type -> Prop :=
+  | Type_le : forall s1 s2 p1 p2,
+      base_type_le s1 s2 ->
+      policy_le p1 p2 ->
+      type_le (Typ s1 p1) (Typ s2 p2)
+
+  with base_type_le : base_type -> base_type -> Prop :=
+  | Base_type_le_refl : forall s, base_type_le s s
+  | Base_type_le_lambda : forall G1 G1' G2 G2' k u p1 p2 md k',
+      policy_le p2 p1 ->
+      context_le G2 G1 ->
+      context_le G1' G2' ->
+      base_type_le (Tlambda G1 k u p1 md G1' k')
+                   (Tlambda G2 k u p2 md G2' k')
+
+  with context_le : context -> context -> Prop :=
+  | Context_le : forall G1 G2,
+      (forall x t,
+          var_in_dom G1 x t -> exists t',
+            var_in_dom G2 x t' /\ type_le t t') ->
+      (forall x t,
+          var_in_dom G2 x t -> exists t', var_in_dom G1 x t') ->
+      (forall l t rt,
+          loc_in_dom G1 l t rt -> exists t',
+            loc_in_dom G2 l t' rt /\ type_le t t') ->
+      (forall l t rt,
+          loc_in_dom G2 l t rt -> exists t', loc_in_dom G1 l t' rt) ->
+      context_le G1 G2.
+
+  Definition context_wt (G: context) (d: loc_mode) : Prop :=
+    forall_loc G (fun l t _ =>
+                    let (_, p) := t in
+                    p <> LevelP T /\ (p = LevelP H -> exists i, d l = Encl i)).
+  
+  Definition is_var_low_context (G: context) : Prop :=
+    forall_var G (fun _ t => let (_, p) := t in p = LevelP L).
+
+  Definition all_loc_immutable (e: exp2) (G: context) : Prop :=
+    forall_subexp2 e (fun e =>
+                       match e with
+                       | Eloc (Cnd _) => False
+                       | Eloc (Not_cnd l) => forall t rt,
+                           loc_context G (Not_cnd l) = Some (t, rt) ->
+                           rt = Immut
+                       | _ => True
+                       end).
+
+  (* FIXME: don't have subsumption rule *)
+  Inductive exp2_type : mode -> context -> loc_mode -> exp2 -> type -> Prop :=
+  | ETnat : forall md g d n,
+      exp2_type md g d (Enat n) (Typ Tnat (LevelP L))
+  | ETvar : forall md g d x t,
+      var_context g x = Some t -> exp2_type md g d (Evar x) t
+  | ETcnd : forall md g d a md',
+      let l := Cnd a in
+      d l = md' ->
+      exp2_type md g d (Eloc l) (Typ (Tcond md') (LevelP L))
+  | ETloc : forall md g d a md' t rt,
+      let l := Not_cnd a in
+      d l = md' ->
+      loc_context g l = Some (t, rt) ->
+      exp2_type md g d (Eloc l) (Typ (Tref t md' rt) (LevelP L))
+  | ETderef : forall md g d e md' s p rt q,
+      exp2_type md g d e (Typ (Tref (Typ s p) md' rt) q) ->
+      md' = Normal \/ md' = md ->
+      exp2_type md g d (Ederef e) (Typ s (policy_join p q))
+  | ETunset : forall md g d cnd md',
+      md' = d (Cnd cnd) ->
+      md' = Normal \/ md' = md ->
+      exp2_type md g d (Eisunset cnd) (Typ Tnat (LevelP L))
+  | ETlambda : forall md g d c p k u g' k',
+      com2_type p md g k u d c g' k' ->
+      exp2_type md g d (Elambda md c) (Typ (Tlambda g k u p md g' k') (LevelP L))
+  | ETplus : forall md g d e1 e2 p q,
+      exp2_type md g d e1 (Typ Tnat p) ->
+      exp2_type md g d e2 (Typ Tnat q) ->
+      exp2_type md g d (Eplus e1 e2) (Typ Tnat (policy_join p q))
+  | ETmult : forall md g d e1 e2 p q,
+      exp2_type md g d e1 (Typ Tnat p) ->
+      exp2_type md g d e2 (Typ Tnat q) ->
+      exp2_type md g d (Emult e1 e2) (Typ Tnat (policy_join p q))
+
+  with com2_type : sec_policy -> mode -> context -> set enclave ->
+                  set condition -> loc_mode -> com2 ->
+                  context -> set enclave -> Prop :=
+  | CTskip : forall pc md g d k u,
+      mode_alive md k ->
+      com2_type pc md g k u d Cskip g k
+  | CTkill : forall i g d k u,
+      mode_alive (Encl i) k ->
+      com2_type (LevelP L) Normal g k u d (Ckill i) g (set_add Nat.eq_dec i k)
+  | CTassign : forall pc md g k u d x e s p q vc lc vc',
+      exp2_type md g d e (Typ s p) ->
+      q = policy_join p pc ->
+      q <> LevelP T ->
+      policy_le q (LevelP L) \/ md <> Normal ->
+      mode_alive md k ->
+      g = Cntxt vc lc ->
+      vc' = (fun y => if y =? x then Some (Typ s q) else vc y) ->
+      com2_type pc md g k u d (Cassign x e) (Cntxt vc' lc) k
+  | CTdeclassify : forall md g k u d x e s p vc lc vc',
+      exp2_type md g d e (Typ s p) ->
+      p <> LevelP T ->
+      mode_alive md k ->
+      exp2_novars e ->
+      all_loc_immutable e g ->
+      vc' = (fun y => if y =? x then Some (Typ s (LevelP L)) else vc y) ->
+      com2_type (LevelP L) md g k u d (Cdeclassify x e) (Cntxt vc' lc) k
+  | CToutput : forall pc md g k u d e l s p,
+      exp2_type md g d e (Typ s p) ->
+      mode_alive md k ->
+      p <> LevelP T ->
+      sec_level_le (sec_level_join (cur p u) (cur pc u)) l ->
+      com2_type pc md g k u d (Coutput e l) g k
+  | CTupdate : forall pc md g k u d e1 e2 s p md' q p',
+      exp2_type md g d e1 (Typ (Tref (Typ s p) md' Mut) q) ->
+      exp2_type md g d e2 (Typ s p') ->
+      policy_le (policy_join (policy_join p' q) pc) p ->
+      md' = Normal \/ md' = md ->
+      mode_alive md k ->
+      p <> LevelP T ->
+      p' <> LevelP T ->
+      q <> LevelP T ->
+      com2_type pc md g k u d (Cupdate e1 e2) g k
+  | Tset : forall md g k u d cnd md',
+      md' = d (Cnd cnd) ->
+      ~set_In cnd u ->
+      md' = Normal \/ md' = md ->
+      mode_alive md k ->
+      com2_type (LevelP L) md g k u d (Cset cnd) g k
+  | Tifunset : forall pc md g k u d cnd c1 c2 g' k',
+      exp2_type md g d (Eisunset cnd) (Typ Tnat (LevelP L)) ->
+      com2_type pc md g k (set_add Nat.eq_dec cnd u) d c1 g' k' ->
+      com2_type pc md g k u d c2 g' k' ->
+      com2_type pc md g k u d (Cif (Eisunset cnd) c1 c2) g' k'
+  | Tifelse : forall pc md g k u d e c1 c2 pc' p g' k',
+      ~(exists cnd, e = Eisunset cnd) ->
+      com2_type pc' md g k u d c1 g' k' ->
+      com2_type pc' md g k u d c2 g' k' ->
+      exp2_type md g d e (Typ Tnat p) ->
+      policy_le (policy_join pc p) pc' ->
+      policy_le p (LevelP L) \/ md <> Normal ->
+      p <> LevelP T ->
+      com2_type pc md g k u d (Cif e c1 c2) g' k'
+  | Tenclave : forall pc g k u d c i c' g' k',
+      c = Cenclave i c' ->
+      com2_type pc (Encl i) g k nil d c' g' k' ->
+      is_var_low_context g' ->
+      com2_type pc Normal g k u d c g' k'
+  | Twhile : forall pc md g k u d c e p pc',
+      exp2_type md g d e (Typ Tnat p) ->
+      com2_type pc' md g k u d c g k ->
+      policy_le (policy_join pc p) pc' ->
+      policy_le p (LevelP L) \/ md <> Normal ->
+      p <> LevelP T ->
+      com2_type pc md g k u d (Cwhile e c) g k
+  | Tseq : forall pc md g k u d c rest g' k' gn kn,
+      com2_type pc md g k u d c g' k' ->
+      com2_type pc md g' k' u d (Cseq rest) gn kn ->
+      com2_type pc md g k u d (Cseq (c :: rest)) gn kn
+  | Tseqnil : forall pc md g k u d,
+      com2_type pc md g k u d (Cseq []) g k
+  | Tcall : forall pc md G u d e Gm km Gp kp Gout q p,
+      exp2_type md G d e (Typ (Tlambda Gm km u p md Gp kp) q) ->
+      policy_le (policy_join pc q) p ->
+      q <> LevelP T ->
+      u = nil \/ md <> Normal ->
+      forall_dom Gm
+                 (fun x t => exists t', var_in_dom G x t' /\ type_le t' t)
+                 (fun l t rt => exists t',
+                      loc_in_dom G l t' rt /\ type_le t' t) ->
+      forall_dom Gp
+                 (fun x t => exists t', var_in_dom Gout x t' /\ type_le t' t)
+                 (fun l t rt => exists t',
+                      loc_in_dom Gout l t' rt /\ type_le t' t) ->
+      forall_dom G
+                 (fun x t =>
+                    (forall t', ~var_in_dom Gp x t') ->
+                    var_in_dom Gout x t)
+                 (fun l t rt =>
+                    (forall t' rt', ~loc_in_dom Gp l t' rt') ->
+                    loc_in_dom Gout l t rt) ->
+      com2_type pc md G km u d (Ccall e) Gout kp.
+  
+End Typing.
+
+Section Security.
+  Inductive protected : sec_policy -> set condition -> Prop :=
+  | level_high: forall S, protected (LevelP H) S
+  | level_top: forall S, protected (LevelP T) S
+  | erase_high: forall cnd S sl, protected (ErasureP H cnd sl) S
+  | erase_low: forall cnd S sl, protected (ErasureP L cnd sl) S.
+      
+  Definition overlap (tr tobs: trace) :=
+  | tobs is entirely contained in tr => tobs
+  | tobs is after tr => empty
+  | overlap with beginning of tobs => beginning of tobs
+                                                    
+  Lemma eq_overlap_tobs (m1 m2: mem) (tobs: trace) :
+    forall md d c k r' m' k' tr1 tr2,
+    cstep md d (c, reg_init, m1, k) (r', m', k') tr1 ->
+    cstep md d (c, reg_init, m2, k) (r', m', k') tr2 ->
+    tobs_sec_level L (overlap tr1 tobs) = tobs_sec_level L (overlap tr2 tobs).
+      
+End Security.
